Commit misc and trivial updates to several files

pancake/crep_to_loopScript.sml
@@ -94,82 +94,80 @@ Definition rt_var_def:
 End
 
 
-Definition compile_prog_def:
-  (compile_prog _ _ (Skip:'a crepLang$prog) = (Skip:'a loopLang$prog)) /\
-  (compile_prog _ _ Break = Break) /\
-  (compile_prog _ _ Continue = Continue) /\
-  (compile_prog _ _ Tick = Tick) /\
-  (compile_prog ctxt l (Return e) =
+Definition compile_def:
+  (compile _ _ (Skip:'a crepLang$prog) = (Skip:'a loopLang$prog)) /\
+  (compile _ _ Break = Break) /\
+  (compile _ _ Continue = Continue) /\
+  (compile _ _ Tick = Tick) /\
+  (compile ctxt l (Return e) =
     let (p, le, ntmp, nl) = compile_exp ctxt (ctxt.vmax + 1) l e in
       nested_seq (p ++ [Assign ntmp le; Return ntmp])) /\
-  (compile_prog ctxt l (Raise eid) =
+  (compile ctxt l (Raise eid) =
     Seq (Assign (ctxt.vmax + 1) (Const eid)) (Raise (ctxt.vmax + 1))) /\
-  (compile_prog ctxt l (Store dst src) =
+  (compile ctxt l (Store dst src) =
     let (p, le, tmp, l) = compile_exp ctxt (ctxt.vmax + 1) l dst in
       let (p', le', tmp, l) = compile_exp ctxt tmp l src in
         nested_seq (p ++ p' ++ [Assign tmp le'; Store le tmp])) /\
-  (compile_prog ctxt l (StoreByte dst src) =
+  (compile ctxt l (StoreByte dst src) =
     let (p, le, tmp, l) = compile_exp ctxt (ctxt.vmax + 1) l dst in
       let (p', le', tmp, l) = compile_exp ctxt tmp l src in
         nested_seq (p ++ p' ++
                      [Assign tmp le; Assign (tmp + 1) le';
                       StoreByte tmp (tmp + 1)])) /\
-  (compile_prog ctxt l (StoreGlob adr e) =
+  (compile ctxt l (StoreGlob adr e) =
     let (p, le, tmp, l) = compile_exp ctxt (ctxt.vmax + 1) l e in
         nested_seq (p ++ [SetGlobal adr le])) /\
-  (compile_prog ctxt l (Seq p q) =
-    Seq (compile_prog ctxt l p) (compile_prog ctxt l q)) /\
-  (compile_prog ctxt l (Assign v e) =
+  (compile ctxt l (Seq p q) =
+    Seq (compile ctxt l p) (compile ctxt l q)) /\
+  (compile ctxt l (Assign v e) =
     case FLOOKUP ctxt.vars v of
      | SOME n =>
        let (p,le,tmp, l) = compile_exp ctxt (ctxt.vmax + 1) l e in
         nested_seq (p ++ [Assign n le])
      | NONE => Skip) /\
-  (compile_prog ctxt l (Dec v e prog) =
+  (compile ctxt l (Dec v e prog) =
     let (p,le,tmp,nl) = compile_exp ctxt (ctxt.vmax + 1) l e;
          nctxt = ctxt with <|vars := ctxt.vars |+ (v,tmp);
                              vmax := tmp|>;
          fl = insert tmp () l;
-         lp = compile_prog nctxt fl prog in
+         lp = compile nctxt fl prog in
      Seq (nested_seq p) (Seq (Assign tmp le) lp)) /\
-  (compile_prog ctxt l (If e p q) =
+  (compile ctxt l (If e p q) =
     let (np, le, tmp, nl) = compile_exp ctxt (ctxt.vmax + 1) l e;
-        lp = compile_prog ctxt l p;
-        lq = compile_prog ctxt l q in
+        lp = compile ctxt l p;
+        lq = compile ctxt l q in
     nested_seq (np ++ [Assign tmp le;
                        If NotEqual tmp (Imm 0w) lp lq l])) /\
 
-  (compile_prog ctxt l (While e p) =
+  (compile ctxt l (While e p) =
     let (np, le, tmp, nl) = compile_exp ctxt (ctxt.vmax + 1) l e;
-        lp = compile_prog ctxt l p in
+        lp = compile ctxt l p in
      Loop l (nested_seq (np ++ [
                 Assign tmp le;
                 If NotEqual tmp (Imm 0w)
                    (Seq lp Continue) Break l]))
           l) /\
-  (compile_prog ctxt l (Call Tail e es) =
+  (compile ctxt l (Call Tail e es) =
    let (p, les, tmp, nl) = compile_exps ctxt (ctxt.vmax + 1) l (es ++ [e]);
        nargs = gen_temps tmp (LENGTH les) in
    nested_seq (p ++ MAP2 Assign nargs les ++
                [Call NONE NONE nargs NONE])) /\
-
-
-  (compile_prog ctxt l (Call (Ret rt rp hdl) e es) =
+  (compile ctxt l (Call (Ret rt rp hdl) e es) =
    let (p, les, tmp, nl) = compile_exps ctxt (ctxt.vmax + 1) l (es ++ [e]);
        nargs = gen_temps tmp (LENGTH les);
        rn  = rt_var ctxt.vars rt (ctxt.vmax + 1) (ctxt.vmax + 1);
        en  = ctxt.vmax + 1;
-       pr  = compile_prog ctxt l rp;
+       pr  = compile ctxt l rp;
        pe  = case hdl of
               | NONE => Raise en
               | SOME (Handle eid ep) =>
-                let cpe = compile_prog ctxt l ep in
+                let cpe = compile ctxt l ep in
                 if ~MEM eid ctxt.ceids then (Raise en)
                 else (If NotEqual en (Imm eid) (Raise en) (Seq Tick cpe) l) in
       nested_seq (p ++ MAP2 Assign nargs les ++
                [Call (SOME (rn, l)) NONE nargs
                      (SOME (en, pe, pr, l))])) /\
-  (compile_prog ctxt l (ExtCall f ptr1 len1 ptr2 len2) =
+  (compile ctxt l (ExtCall f ptr1 len1 ptr2 len2) =
     case (FLOOKUP ctxt.vars ptr1, FLOOKUP ctxt.vars len1,
           FLOOKUP ctxt.vars ptr2, FLOOKUP ctxt.vars len2) of
      | (SOME pc, SOME lc, SOME pc', SOME lc') =>
