pancake/loop_to_loopremoveScript.sml
@@ -90,16 +90,4 @@ Definition comp_with_loop_def:
   (comp_with_loop p prog cont s = (Fail,s)) (* impossible case *)
 End
 
-Definition comp_def:
-  comp (name,params,prog) s =
-    let (body,n,funs) = comp_with_loop (Fail,Fail) prog Fail s in
-      (n,(name,params,body)::funs)
-End
-
-Definition comp_all_def:
-  comp_all code =
-    let n = FOLDR MAX 0 (MAP FST code) + 1 in
-      SND (FOLDR comp (n,[]) code)
-End
-
 val _ = export_theory();
