pancake/proofs/loop_removeProofScript.sml
@@ -7,170 +7,18 @@ local open wordSemTheory in end
 
 val _ = new_theory"loop_removeProof";
 
-Definition mark_all_def:
-  (mark_all (Seq p1 p2) =
-     let (p1,t1) = mark_all p1 in
-     let (p2,t2) = mark_all p2 in
-     let t3 = (t1 /\ t2) in
-       (if t3 then Mark (Seq p1 p2) else Seq p1 p2, t3)) /\
-  (mark_all (Loop l1 body l2) =
-     let (body,t1) = mark_all body in
-       (Loop l1 body l2, F)) /\
-  (mark_all (If x1 x2 x3 p1 p2 l1) =
-     let (p1,t1) = mark_all p1 in
-     let (p2,t2) = mark_all p2 in
-     let p3 = If x1 x2 x3 p1 p2 l1 in
-     let t3 = (t1 /\ t2) in
-       (if t3 then Mark p3 else p3, t3)) /\
-  (mark_all (Mark p1) = mark_all p1) /\
-  (mark_all (Call ret dest args handler) =
-     case handler of
-     | NONE => (Mark (Call ret dest args handler), T)
-     | SOME (n,p1,p2,l) =>
-         let (p1,t1) = mark_all p1 in
-         let (p2,t2) = mark_all p2 in
-         let t3 = (t1 ∧ t2) in
-         let p3 = Call ret dest args (SOME (n,p1,p2,l)) in
-           (if t3 then Mark p3 else p3, t3)) /\
-  (mark_all prog = (Mark prog,T))
-End
-
-Theorem mark_all_syntax_ok:
-  ∀prog q b.
-     mark_all prog = (q,b) ==>
-     b = no_Loop q ∧ syntax_ok q
-Proof
-  recInduct mark_all_ind \\ rpt conj_tac
-  \\ rpt gen_tac \\ strip_tac
-  THEN1
-   (fs [mark_all_def]
-    \\ rpt (pairarg_tac \\ fs []) \\ rveq
-    \\ IF_CASES_TAC
-    \\ fs [evaluate_def,every_prog_def,no_Loop_def,syntax_ok_def])
-  THEN1
-   (fs [mark_all_def]
-    \\ rpt (pairarg_tac \\ fs []) \\ rveq
-    \\ fs [every_prog_def,no_Loop_def,syntax_ok_def])
-  THEN1
-   (fs [mark_all_def]
-    \\ rpt (pairarg_tac \\ fs []) \\ rveq
-    \\ IF_CASES_TAC \\ fs []
-    \\ fs [no_Loop_def,every_prog_def,syntax_ok_def])
-  THEN1 fs [mark_all_def,syntax_ok_def]
-  THEN1
-   (fs [mark_all_def] \\ rveq
-    \\ every_case_tac \\ fs []
-    \\ fs [no_Loop_def,every_prog_def,syntax_ok_def]
-    \\ rpt (pairarg_tac \\ fs []) \\ rveq
-    \\ IF_CASES_TAC \\ fs []
-    \\ fs [every_prog_def,syntax_ok_def,no_Loop_def])
-  \\ fs [mark_all_def] \\ rveq
-  \\ fs [every_prog_def,no_Loop_def,syntax_ok_def]
-QED
-
-Theorem mark_all_evaluate:
-  ∀prog q b.
-     mark_all prog = (q,b) ==>
-     ∀s. evaluate (prog,s) = evaluate (q,s)
-Proof
-  recInduct mark_all_ind \\ rpt conj_tac
-  \\ rpt gen_tac \\ strip_tac
-  THEN1
-   (fs [mark_all_def]
-    \\ rpt (pairarg_tac \\ fs []) \\ rveq
-    \\ IF_CASES_TAC \\ fs [evaluate_def])
-  THEN1
-   (fs [mark_all_def]
-    \\ rpt (pairarg_tac \\ fs []) \\ rveq
-    \\ match_mp_tac evaluate_Loop_body_same \\ fs [])
-  THEN1
-   (fs [mark_all_def]
-    \\ rpt (pairarg_tac \\ fs []) \\ rveq
-    \\ IF_CASES_TAC \\ fs []
-    \\ fs [every_prog_def,evaluate_def]
-    \\ fs [no_Loop_def,every_prog_def]
-    \\ rw [] \\ every_case_tac \\ fs [])
-  THEN1 fs [mark_all_def,evaluate_def]
-  THEN1
-   (fs [mark_all_def] \\ rveq
-    \\ every_case_tac \\ fs []
-    \\ fs [no_Loop_def,every_prog_def,evaluate_def]
-    \\ rpt (pairarg_tac \\ fs []) \\ rveq
-    \\ IF_CASES_TAC \\ fs []
-    \\ fs [every_prog_def,evaluate_def])
-  \\ fs [mark_all_def] \\ rveq
-  \\ simp [evaluate_def]
-  \\ fs [every_prog_def,no_Loop_def]
-QED
-
-Definition comp_no_loop_def:
-  (comp_no_loop p (Seq p1 p2) =
-    Seq (comp_no_loop p p1) (comp_no_loop p p2)) /\
-  (comp_no_loop p (If x1 x2 x3 p1 p2 l1) =
-    If x1 x2 x3 (comp_no_loop p p1) (comp_no_loop p p2) l1) /\
-  (comp_no_loop p (Call ret dest args handler) =
-    Call ret dest args
-      (case handler of
-       | SOME (n,q,r,l) => SOME (n, comp_no_loop p q, comp_no_loop p r, l)
-       | NONE => NONE)) /\
-  (comp_no_loop p Break = FST p) /\
-  (comp_no_loop p Continue = SND p) /\
-  (comp_no_loop p (Mark prog) = comp_no_loop p prog) /\
-  (comp_no_loop p (Loop l1 b l2) = Fail) /\
-  (comp_no_loop p prog = prog)
-End
-
-Definition store_cont_def:
-  store_cont live code (n,funs) =
-    let params = MAP FST (toSortedAList live) in
-    let funs = (n,params,code) :: funs in
-    let cont = Call NONE (SOME n) params NONE in
-      (cont:'a loopLang$prog, (n+1,funs))
-End
-
-Definition comp_with_loop_def:
-  (comp_with_loop p (Seq p1 p2) cont s =
-     let (q2,s) = comp_with_loop p p2 cont s in
-       comp_with_loop p p1 q2 s) ∧
-  (comp_with_loop p (If x1 x2 x3 p1 p2 l1) cont s =
-     let (cont,s) = store_cont l1 cont s in
-     let (q1,s) = comp_with_loop p p1 cont s in
-     let (q2,s) = comp_with_loop p p2 cont s in
-       (If x1 x2 x3 q1 q2 LN,s)) /\
-  (comp_with_loop p (Call ret dest args handler) cont s =
-     case handler of
-     | NONE => (Seq (Call ret dest args NONE) cont,s)
-     | SOME (n,q,r,l) =>
-         let (cont,s) = store_cont l cont s in
-         let (q,s) = comp_with_loop p q cont s in
-         let (r,s) = comp_with_loop p r cont s in
-           (Call ret dest args (SOME (n,q,r,l)),s)) /\
-  (comp_with_loop p Break cont s = (FST p,s)) /\
-  (comp_with_loop p Continue cons s = (SND p,s)) /\
-  (comp_with_loop p (Mark prog) cont s = (Seq (comp_no_loop p prog) cont,s)) /\
-  (comp_with_loop p (Loop live_in body live_out) cont s =
-     let (cont,s) = store_cont live_out cont s in
-     let params = MAP FST (toSortedAList live_in) in
-     let (n,funs) = s in
-     let enter = Call NONE (SOME n) params NONE in
-     let (body,m,funs) = comp_with_loop (cont,enter) body Fail (n+1,funs) in
-     let funs = (n,params,body) :: funs in
-       (enter,(m,funs))) ∧
-  (comp_with_loop p prog cont s = (Fail,s)) (* impossible case *)
-End
-
 Definition comp_def:
   comp (name,params,prog) s =
     let (body,n,funs) = comp_with_loop (Fail,Fail) prog Fail s in
       (n,(name,params,body)::funs)
 End
-
+(*
 Definition comp_all_def:
   comp_all code =
     let n = FOLDR MAX 0 (MAP FST code) + 1 in
       SND (FOLDR comp (n,[]) code)
 End
-
+*)
 Definition has_code_def:
   has_code (n,funs) code =
     EVERY (\(n,p,b). lookup n code = SOME (p,b)) funs
